subst_help

proofs.v
@@ -1,19 +1,12 @@
 Require Import Program.Equality Ring.
 From mathcomp Require Import ssreflect ssrfun ssrbool seq eqtype ssrnat.
-From istari Require Import source subst_src rules_src help trans basic_types.
+From istari Require Import source subst_src rules_src help subst_help trans basic_types.
 From istari Require Import Sigma Tactics
      Syntax Subst SimpSub Promote Hygiene
      ContextHygiene Equivalence Rules Defined.
-Check context.
+
 Ltac var_solv :=
   try (apply tr_hyp_tm; repeat constructor).
-
-Ltac simpsub_backup := repeat (try rewrite subst_laters; try rewrite subst_subseq; try rewrite subst_store;
-        try rewrite subst_pw;
-        try rewrite subst_nzero; try rewrite subst_nat; try rewrite subst_pw; simpsub; simpl).
-
-Ltac simpsub_big := repeat (simpsub; simpsub1).
-
 
 Lemma tr_arrow_elim: forall G a b m n p q, 
     tr G (deqtype a a) ->
@@ -60,9 +53,6 @@ Hint Resolve nat_U0.
 Lemma nat_type: forall G,
       tr G (deqtype nattp nattp). Admitted.
 Hint Resolve nat_type. 
-
-
-
 
 Lemma pw_kind: forall {G},
     tr G (deq preworld preworld (kuniv nzero)).
@@ -342,16 +332,6 @@ Lemma bind_type: forall G A B M0 M1,
     tr G (oof M1 (arrow A (laters B))) ->
     tr G (oof (make_bind M0 M1) (laters B)). Admitted.
 
-Lemma sh_sum :
-  forall m n t,
-    @subst False (sh n) (subst (sh m) t) = @subst False (sh (n+m)) t.
-  intros. repeat rewrite subst_sh_shift.
-  rewrite shift_sum. auto. Qed.
-
-Lemma shh_sum :
-  forall m n t,
-    @substh False (sh n) (substh (sh m) t) = @substh False (sh (n+m)) t.
-Admitted.
 
 Lemma world_pair: forall w l G, tr G (oof w preworld) ->
                            tr G (oof l nattp) ->
@@ -498,7 +478,6 @@ repeat rewrite - addnA;
     rewrite subst_lt. simpsub. auto.
 Qed.
 
-(*pick up here*)
 Lemma compm4_type: forall U A G,
     (tr G (oof U world)) ->
     (tr [:: hyp_tm nattp, hyp_tm preworld & G] (oof A U0)) ->
@@ -771,9 +750,6 @@ Opaque nattp.
 Opaque world.
 Opaque nth.*)
 
-Theorem test: forall s, (@subst False s nattp) = nattp.
-  intros. simpsub1. Admitted.
-
 (*Theorem one_five: forall G D e T ebar w1 l1, 
     of_m G e T ->
     trans e ebar -> 
@@ -826,308 +802,6 @@ Lemma wworld_app: forall G D w1 l1,
   intros. eapply tr_weakening_appends; try apply X; try reflexivity; auto.
   rewrite - subst_sh_shift. auto.
   rewrite - subst_sh_shift. auto. Qed.
-
-(*Definition gen_sub G s := foldr (fun _  => fun s => )*)
-
-
-Lemma test1: forall (t: term False), subst (dot (var 1) (dot (var 0) (sh 2)))
-                                  (subst (under 1 (dot (var 1) (dot (var 0) (sh 2)))) t) =
-                            subst (gen_sub_mvl 2) t.
-intros. simpl. simpsub. simpl. auto. Qed.
-
-
-(*Lemma test2:
-  @subst False (dot (var 0) (sh 2)) (ppair (var 0)
-                                    (var 1)
-                             ) = subst sh1 (ppair (var 0)
-                                    (var 1)
-                                           ).
-  simpsub. simpl.*)
-
-Lemma substctx_eqsub {s s': @sub False} {G: context}
-: eqsub s s'
-    -> substctx s G = substctx s' G. Admitted.
-
-(*Lemma test1: forall (t: term False), subst (dot (var 1) (dot (var 0) (sh 2)))
-                       (subst (under 1 (dot (var 1) (dot (var 0) (sh 2)))) t) =
-                            t.
-  intros. simpsub. ring.*)
-
-(*start here*)
-(*IDEA: do the move when there's only one variable to move: before 72*)
-
-
-
-Lemma substctx_app: forall G1 G2 s,
-    @substctx False s (G1 ++ G2) = (substctx (under (size G2) s) G1) ++ (substctx s G2).
-  intros. induction G1; simpsub. repeat rewrite cat0s. auto.
-  simpl. simpsub. repeat rewrite plusE.
-  replace ((length G1) + (size G2)) with (size (G1 ++ G2)).
-  rewrite - IHG1. auto.
-  rewrite size_cat. auto. Qed.
-
-Lemma substctx_rcons: forall G1 g s,
-    @substctx False s (rcons G1 g) = rcons (substctx (under 1 s) G1) (substh s g).
-  intros. repeat rewrite - cats1. rewrite substctx_app. simpl. auto. Qed.
-
-
-(*induction G; simpsub. auto.
-  simpl. move: IHG. simpsub. move => IHG. simpl. auto.
-  rewrite IHG.
-  suffices: (@eqsub False (dot (var 0) (sh 2)) sh1).
-  move/(eqsub_under _ (length G)) => Heqsub.
-  rewrite (substh_eqsub _ _ _ _ Heqsub). auto.
-  intros b c. induction b; simpsub.
-  .
-  rewrite - (sh_sum 1 1).*)
-
-
-Lemma size_substctx :
-  forall s G, size (@substctx False s G) = size G.
-Proof.
-  intros. move: (length_substctx False s G). apply.
-Qed.
-
-Hint Rewrite size_substctx.
-
-Lemma move_var_r: forall E v G D m m' a,
-    tr ((substctx (gen_sub_mvr (size G)) E) ++ (substctx (sh1) G) ++ v::D) (deq m m'
-                                         (subst (under (size E) (gen_sub_mvr (size G))) a)
-                                                               ) ->
-    tr (E ++ ((substh (sh (size G)) v):: (G ++ D))) (deq (subst (under (size E) (gen_sub_mvl (size G))) m)
-                               (subst (under (size E) (gen_sub_mvl (size G))) m')
-                               a).
-  move => E v G. move: E v. induction G using last_ind; intros. move: X.
-  simpl. unfold gen_sub_mvl. simpl. unfold sh1. simpsub. auto.
-  (*suffices: @ eqsub False id (dot (var 0) sh1). move => Heq. remember Heq as Heq1.
-  clear HeqHeq1. move/eqsub_under : Heq1 => Heq1.
-  rewrite - !(subst_eqsub _ _ _ _ (Heq1 (size E))) - !(substctx_eqsub _ _ _ Heq). simpsub. auto. *)
-  - rewrite size_rcons. simpl. rewrite !compose_under !subst_compose.
-    rewrite - 1!(addn1 (size G)). rewrite - shh_sum.
-    rewrite cat_rcons.
-    eapply IHG.
-    rewrite catA. rewrite under_sum. rewrite !plusE.
-    replace (size E + size G) with
-        (size (substctx (gen_sub_mvr (size G)) E ++ substctx sh1 G)).
-    apply tr_exchange.
-    rewrite substctx_app.
-    repeat rewrite size_substctx. rewrite - substctx_compose.
-    replace (substctx
-        (compose (gen_sub_mvr (size G))
-           (under (size G)
-                  (dot (var 1) (dot (var 0) (sh 2))))) E) with
-        (substctx (gen_sub_mvr (size (rcons G x))) E).
-    rewrite substctx_mvr.
-    suffices: (((substctx (gen_sub_mvr (size (rcons G x))) E) ++
-      substctx (under 1 sh1) G) ++
-                                [:: substh sh1 x, v & D])%list=
-((substctx (gen_sub_mvr (size (rcons G x))) E) ++
-                                                   (rcons (substctx (under 1 sh1) G) (substh sh1 x)) ++ [:: v & D]).
-    move => Heq. rewrite Heq. rewrite - (cats1 _ (substh sh1 x)).
-    replace (substctx (under 1 sh1) G ++ [:: substh sh1 x]) with
-        (substctx sh1 (rcons G x)).
-    replace 
-       (subst
-          (under
-             (length
-                (substctx
-                   (gen_sub_mvr
-                      (size G)) E ++
-                 substctx sh1 G))
-             (dot (var 1)
-                (dot (var 0) (sh 2))))
-          (subst
-             (under (size E)
-                (gen_sub_mvr
-                   (size G))) a))
- with
-           (subst
-              (under (size E)
-                     (gen_sub_mvr (size (rcons G x)))) a). apply X.
-    rewrite size_rcons. simpl. rewrite List.app_length.
-    repeat rewrite length_substctx.
-    rewrite compose_under. rewrite under_sum.
-    rewrite - subst_compose. auto.
-    rewrite - cats1. rewrite substctx_app. simpl. auto.
-    rewrite - (cats1 _ (substh sh1 x)).
-    rewrite - catA. rewrite (cat1s _ (v::D)). auto.
-    rewrite catA. auto.
-    rewrite size_rcons. auto.
-    rewrite size_cat. repeat rewrite size_substctx. auto.
-Qed.
-
-Fixpoint gen_sub_mvl_list g v :=
-  match v with
-    0 => id
-          | S v' => compose (gen_sub_mvl_list g v') (under v' (gen_sub_mvl g)) end.
-
-Fixpoint gen_sub_mvr_list g v :=
-  match v with
-    0 => id
-          | S v' => compose (under v' (gen_sub_mvr g )) (gen_sub_mvr_list g v') end.
-
-(*Fixpoint gen_sub_mvr_ctx g v :=
-  match v with
-    0 => id
-          | S v' => compose (gen_sub_mvr g ) (gen_sub_mvr_ctx g v') end.*)
-
-(*prove this
- try and implement it practically with trans
-Lemma move_var_r: forall E v G D m m' a,
-    tr ((substctx (gen_sub_mvr (size G)) E) ++ (substctx (sh1) G) ++ v::D) (deq m m'
-                                         (subst (under (size E) (gen_sub_mvr (size G))) a)
-                                                               )
-    -> tr (E ++ ((substh (sh (size G)) v):: (G ++ D))) (deq (subst (under (size E) (gen_sub_mvl (size G))) m)
-                               (subst (under (size E) (gen_sub_mvl (size G))) m')
-                               a).*)
-(*looks a lot like substctx_mvr*)
-Lemma eqsub_project : forall s s',
-  (forall i,
-      project s i = project s' i) ->
-    @eqsub False s s'
-.
-  Admitted. 
-
-
-(*Lemma aa: forall g,
-    project (gen_sub_mvr g) 0 = (var 0).
-  intros. induction g; simpl; simpsub. auto.
-  rewrite IHg. simpsub.
-  suffices:  g = 0.
-  intros. subst. simpsub.
-works for g > 1
-*)
-
-Lemma mvr_works_n0_lt: forall (g i: nat), (i < g ->
-                                 project (gen_sub_mvr g) (S i) = (var i)).
-  intros.
-  move: (mvr_works_nz g i) => [one two]. apply one. assumption. Qed.
-
-Lemma mvr_works_n0_gt: forall (g i: nat), ((i >= g) -> project (gen_sub_mvr g) (S i) = (var (S i))).
-  intros.
-  move: (mvr_works_nz g i) => [one two]. apply two. assumption. Qed.
-
-
-
-  Lemma mvr_shift_help: forall g,
-    eqsub (compose (compose (under 1 (sh g))
-                           (gen_sub_mvr g)) (sh1))
-(compose (under 1 (sh (g + 1)))
-                           (gen_sub_mvr (g + 1))). 
-  intros. induction g.
-  simpl. simpsub. simpl. apply eqsub_refl.
-  apply eqsub_project.
-  intros. simpsub. rewrite plusE.
-induction i. simpl. simpsub.
-  simpl.
-  Opaque compose.
-  simpl. rewrite - addnE. simpl.
-  simpl in IHg. rewrite addnC in IHg. simpl in IHg.
-  repeat rewrite mvr_works0. simpsub.
-  repeat rewrite project_under_eq. simpsub.
-  rewrite plusE.
-replace (1 + (g + 1)) with (g + 1 + 1). auto.
-ring.
-simpsub. rewrite plusE. Opaque addn.
-replace (g.+1 + 1 + i) with ((g+1 +i).+1).
-replace (g.+1 + 1 + 1 + i) with ((g+1 + 1 +i).+1).
-repeat rewrite mvr_works_n0_gt. simpsub. rewrite plusE.
-replace (1 + (g +1 + i).+1) with (g + 1 + 1 + i).+1. auto.
-ring. repeat rewrite addn1. apply ltn_addr.
-apply ltnSn. apply ltn_addr. rewrite addn1. apply ltnSn.
-ring. ring.
-Qed.
-
-
-
-Lemma mvr_shift : forall g,
-    eqsub (compose (under 1 (sh g))
-                   (gen_sub_mvr g)) (sh g).
-  induction g.
-  simpsub. simpl. simpsub. apply (eqsub_symm _ _ _
-                                             (@eqsub_expand_id False)).
-Admitted.
-
-
-Lemma move_list_r: forall E V G D m m' a,
-    tr ((substctx (gen_sub_mvr_list (size G) (size V)) E) ++
-        (substctx (sh (size V)) G) ++ V ++ D) (deq m m'
-                                                   (subst (under (size E)
-                                                      (gen_sub_mvr_list (size G) (size V))) a)
-                                                               ) (*need an under for a i think*)
-    -> tr (E ++ (substctx (sh (size G)) V)++ G ++ D)
-         (deq
-            (subst (under (size E) (gen_sub_mvl_list (size G) (size V))) m)
-            (subst (under (size E)  (gen_sub_mvl_list (size G) (size V))) m')
-                               a).
-  intros. move: m m' a G D E X. induction V using last_ind; intros; move: X; simpl; simpsub.
- apply.
-  repeat rewrite size_rcons. simpl.
-  move => X. rewrite substctx_rcons.
-replace 
-    (E ++
-     rcons (substctx (under 1 (sh (size G))) V)
-       (substh (sh (size G)) x) ++ 
-       G ++ D) with
-    ((E ++ (substctx (under 1 (sh (size G))) V)) ++
-       (substh (sh (size G)) x::
-               (G ++ D))).
-rewrite !compose_under !under_sum !subst_compose !plusE. 
-replace (size E + size V) with
-    (size (E ++
-substctx (under 1 (sh (size G))) V
-    )). apply move_var_r.
-rewrite substctx_app.
-rewrite - substctx_compose. rewrite (substctx_eqsub (mvr_shift (size G)) ).
-replace (size G) with (size (substctx sh1 G)).
-remember (substctx
-        (under (size (substctx (under 1 (sh (size (substctx sh1 G)))) V))
-           (gen_sub_mvr (size (substctx sh1 G)))) E) as E'. 
-replace (size E) with (size E').
-rewrite - catA.
-apply IHV.
-repeat rewrite size_substctx. subst.
-simpsub. rewrite plusE.
-repeat rewrite size_substctx.
-replace 
-       
-       (subst
-          (compose
-             (under
-                (size
-                   (E ++
-                    substctx (dot (var 0) (sh (size G + 1))) V))
-                (gen_sub_mvr (size G)))
-             (under (size E)
-                (gen_sub_mvr_list (size G) (size V)))) a)
- with
-           (subst
-              (under (size E)
-                 (compose
-                    (under 
-                       (size V)
-                       (gen_sub_mvr
-                        (size G)))
-                    (gen_sub_mvr_list
-                       (size G)
-                       (size V)))) a).
-replace 
-    (substctx
-       (compose (under (size V) (gen_sub_mvr (size G)))
-          (gen_sub_mvr_list (size G) (size V))) E ++
-       substctx (sh (1 + size V)) G ++ V ++ x :: D) with
-        (substctx
-           (compose (under (size V) (gen_sub_mvr (size G)))
-              (gen_sub_mvr_list (size G) (size V))) E ++
-         substctx (sh (size V).+1) G ++ rcons V x ++ D).
-apply X.
-rewrite - cats1. rewrite - (catA V [::x]). rewrite cat1s. auto.
-rewrite size_cat. rewrite - under_sum. rewrite - compose_under.
-rewrite size_substctx. auto. subst. 
-rewrite size_substctx. auto.
-rewrite size_substctx. auto.
-rewrite size_cat size_substctx. auto.
-rewrite - catA. rewrite cat_rcons. auto. Qed.
 
 
 Theorem one: forall G D e T ebar w1 l1,
@@ -1623,6 +1297,8 @@ simpsub_big. auto. simpsub.
                 (ppair (ppi1 (var 0))
                    (ppair make_subseq
                           (ppair (picomp3 (var 0)) (picomp4 (var 0)))))))) ).
+(*start here*)
+(*IDEA: do the move when there's only one variable to move: before 72*)
    (*rule 72*)
    eapply (tr_exist_elim _ (subst (sh 1) nzero)
                          (subst (sh 1) preworld) 
