subst_help.v
@@ -1,0 +1,345 @@
+From Coq.Lists Require Import List.
+From mathcomp Require Import ssreflect ssrfun ssrbool seq eqtype ssrnat.
+From istari Require Import source subst_src rules_src help.
+From istari Require Import Sigma Tactics
+     Syntax Subst SimpSub Promote Hygiene
+     ContextHygiene Equivalence Rules Defined.
+
+(*basic substitution stuff*)
+
+Lemma eqsub_project : forall s s',
+  (forall i,
+      project s i = project s' i) ->
+    @eqsub False s s'
+.
+  Admitted. 
+
+Lemma size_substctx :
+  forall s G, size (@substctx False s G) = size G.
+Proof.
+  intros. move: (length_substctx False s G). apply.
+Qed.
+
+Hint Rewrite size_substctx.
+
+Lemma substctx_app: forall G1 G2 s,
+    @substctx False s (G1 ++ G2) = (substctx (under (size G2) s) G1) ++ (substctx s G2).
+  intros. induction G1; simpsub. repeat rewrite cat0s. auto.
+  simpl. simpsub. repeat rewrite plusE.
+  replace ((length G1) + (size G2)) with (size (G1 ++ G2)).
+  rewrite - IHG1. auto.
+  rewrite size_cat. auto. Qed.
+
+Lemma substctx_rcons: forall G1 g s,
+    @substctx False s (rcons G1 g) = rcons (substctx (under 1 s) G1) (substh s g).
+  intros. repeat rewrite - cats1. rewrite substctx_app. simpl. auto. Qed.
+
+Lemma substctx_eqsub {s s': @sub False} {G: context}
+: eqsub s s'
+    -> substctx s G = substctx s' G. Admitted.
+
+Ltac simpsub_big := repeat (simpsub; simpsub1).
+Lemma project_dot_geq :
+  forall t s i, i > 0 ->
+           project (dot t s) i = @project False s (i - 1).
+  Admitted.
+
+Lemma sh_sum :
+  forall m n t,
+    @subst False (sh n) (subst (sh m) t) = @subst False (sh (n+m)) t.
+  intros. repeat rewrite subst_sh_shift.
+  rewrite shift_sum. auto. Qed.
+
+Lemma shh_sum :
+  forall m n t,
+    @substh False (sh n) (substh (sh m) t) = @substh False (sh (n+m)) t.
+Admitted.
+
+(*substitutions for moving variables around in context*)
+Fixpoint gen_sub_mvl G := match G with
+                        0 => id
+                          | n'.+1 =>
+@compose False (under n' (dot (var 1) (dot (var 0) (sh 2)))) (gen_sub_mvl n')
+                                    end.
+
+Fixpoint gen_sub_mvr E := match E with
+                        0 => id
+    | n'.+1 => @compose False (gen_sub_mvr n')
+(under n' (dot (var 1) (dot (var 0) (sh 2))))
+                          end.
+
+Fixpoint gen_sub_mvl_list g v :=
+  match v with
+    0 => id
+          | S v' => compose (gen_sub_mvl_list g v') (under v' (gen_sub_mvl g)) end.
+
+Fixpoint gen_sub_mvr_list g v :=
+  match v with
+    0 => id
+          | S v' => compose (under v' (gen_sub_mvr g )) (gen_sub_mvr_list g v') end.
+
+Lemma mvr_works0: forall (g: nat), project (gen_sub_mvr g) 0 = (var g).
+  intros. induction g; simpl.
+  simpsub. auto.
+  simpsub. rewrite IHg. simpsub.
+  destruct (0 == g) eqn: Hbool. move/ eqP : Hbool => Hbool; subst. 
+  simpsub.  auto.
+rewrite project_under_eq. simpsub. rewrite plusE. rewrite addn1. auto.
+Qed.
+
+
+Lemma mvr_works_nz: forall (g i: nat), (i < g ->
+                                 project (gen_sub_mvr g) (S i) = (var i))
+/\ ((i >= g) -> project (gen_sub_mvr g) (S i) = (var (S i))).
+  move => g. induction g; simpl; intros; split; intros. discriminate H. 
+  simpsub. auto.
+  simpsub. move: (IHg i) => [IH1 IH2].
+  destruct (i < g) eqn: Hbool.
+  - rewrite IH1. rewrite subst_var. rewrite project_under_lt. auto.
+    apply/ltP. rewrite Hbool; try constructor. constructor.
+    suffices: i = g. intros. subst.
+    rewrite IH2. rewrite subst_var. rewrite project_under_geq.
+    rewrite minusE. replace (g.+1 - g) with 1.
+    simpsub. rewrite plusE. rewrite addn0. auto.
+    rewrite subSnn. auto. auto. auto.
+apply anti_leq. apply/ andP. split.
+rewrite - ltnS. assumption. rewrite leqNgt.
+apply / negbT : Hbool.
+  - simpsub. move: (IHg i) => [IH1 IH2]. rewrite IH2. simpsub. rewrite project_under_geq.
+    rewrite - subst_var. rewrite minusE.
+    replace
+(subst (dot (var 1) (dot (var 0) (sh 2)))
+       (varx False (i.+1 - g))) with (@var False (i.+1 - g)). simpsub. 
+    rewrite plusE. simpl. rewrite subnKC. auto.
+    apply ltnW in H.
+    eapply (leq_trans H). auto. simpsub.
+    rewrite project_dot_geq.
+    replace (i.+1 - g - 1) with (i- g).
+    rewrite project_dot_geq. simpsub.
+    simpl. rewrite - 1! (addn2). simpl.
+    replace (i.+1 - g) with (i - g - 1 + 2). auto.
+    rewrite subn1. rewrite addn2. simpl. rewrite prednK.
+    rewrite - addn1. rewrite addnBAC. rewrite addn1. auto.
+    rewrite leq_eqVlt. apply/orP. right. assumption. rewrite subn_gt0.
+    assumption. rewrite subn_gt0.
+    assumption.
+    replace (i.+1 - g - 1) with (i.+1 - (g.+1)).
+    rewrite subSS. auto.
+    rewrite subn1. rewrite subSKn. rewrite subSS. auto.
+    rewrite subn_gt0. eapply (ltn_trans H). auto.
+    apply/ leP. apply leqW. rewrite leq_eqVlt. apply/ orP. right. assumption.
+rewrite leq_eqVlt. apply/ orP. right. assumption.
+Qed.
+
+
+Lemma substctx_mvr: forall G,
+    (substctx (dot (var 1) (dot (var 0) (sh 2))) (substctx sh1 G)) =
+    (@substctx False (under 1 sh1) G).
+  intros. simpsub. auto. Qed.
+
+Lemma mvr_works_n0_lt: forall (g i: nat), (i < g ->
+                                 project (gen_sub_mvr g) (S i) = (var i)).
+  intros.
+  move: (mvr_works_nz g i) => [one two]. apply one. assumption. Qed.
+
+Lemma mvr_works_n0_gt: forall (g i: nat), ((i >= g) -> project (gen_sub_mvr g) (S i) = (var (S i))).
+  intros.
+  move: (mvr_works_nz g i) => [one two]. apply two. assumption. Qed.
+
+Lemma mvr_shift_help: forall g,
+    eqsub (compose (compose (under 1 (sh g))
+                           (gen_sub_mvr g)) (sh1))
+(compose (under 1 (sh (g + 1)))
+                           (gen_sub_mvr (g + 1))). 
+  intros. induction g.
+  simpl. simpsub. simpl. apply eqsub_refl.
+  apply eqsub_project.
+  intros. simpsub. rewrite plusE.
+induction i. simpl. simpsub.
+  simpl.
+  Opaque compose.
+  simpl. rewrite - addnE. simpl.
+  simpl in IHg. rewrite addnC in IHg. simpl in IHg.
+  repeat rewrite mvr_works0. simpsub.
+  repeat rewrite project_under_eq. simpsub.
+  rewrite plusE.
+replace (1 + (g + 1)) with (g + 1 + 1). auto.
+ring.
+simpsub. rewrite plusE. Opaque addn.
+replace (g.+1 + 1 + i) with ((g+1 +i).+1).
+replace (g.+1 + 1 + 1 + i) with ((g+1 + 1 +i).+1).
+repeat rewrite mvr_works_n0_gt. simpsub. rewrite plusE.
+replace (1 + (g +1 + i).+1) with (g + 1 + 1 + i).+1. auto.
+ring. repeat rewrite addn1. apply ltn_addr.
+apply ltnSn. apply ltn_addr. rewrite addn1. apply ltnSn.
+ring. ring.
+Qed.
+
+
+Lemma mvr_shift : forall g,
+    eqsub (compose (under 1 (sh g))
+                   (gen_sub_mvr g)) (sh g).
+  induction g.
+  simpsub. simpl. simpsub. apply (eqsub_symm _ _ _
+                                             (@eqsub_expand_id False)).
+Admitted.
+
+Lemma move_var_r: forall E v G D m m' a,
+    tr ((substctx (gen_sub_mvr (size G)) E) ++ (substctx (sh1) G) ++ v::D) (deq m m'
+                                         (subst (under (size E) (gen_sub_mvr (size G))) a)
+                                                               ) ->
+    tr (E ++ ((substh (sh (size G)) v):: (G ++ D))) (deq (subst (under (size E) (gen_sub_mvl (size G))) m)
+                               (subst (under (size E) (gen_sub_mvl (size G))) m')
+                               a).
+  move => E v G. move: E v. induction G using last_ind; intros. move: X.
+  simpl. unfold gen_sub_mvl. simpl. unfold sh1. simpsub. auto.
+  (*suffices: @ eqsub False id (dot (var 0) sh1). move => Heq. remember Heq as Heq1.
+  clear HeqHeq1. move/eqsub_under : Heq1 => Heq1.
+  rewrite - !(subst_eqsub _ _ _ _ (Heq1 (size E))) - !(substctx_eqsub _ _ _ Heq). simpsub. auto. *)
+  - rewrite size_rcons. simpl. rewrite !compose_under !subst_compose.
+    rewrite - 1!(addn1 (size G)). rewrite - shh_sum.
+    rewrite cat_rcons.
+    eapply IHG.
+    rewrite catA. rewrite under_sum. rewrite !plusE.
+    replace (size E + size G) with
+        (size (substctx (gen_sub_mvr (size G)) E ++ substctx sh1 G)).
+    apply tr_exchange.
+    rewrite substctx_app.
+    repeat rewrite size_substctx. rewrite - substctx_compose.
+    replace (substctx
+        (compose (gen_sub_mvr (size G))
+           (under (size G)
+                  (dot (var 1) (dot (var 0) (sh 2))))) E) with
+        (substctx (gen_sub_mvr (size (rcons G x))) E).
+    rewrite substctx_mvr.
+    suffices: (((substctx (gen_sub_mvr (size (rcons G x))) E) ++
+      substctx (under 1 sh1) G) ++
+                                [:: substh sh1 x, v & D])%list=
+((substctx (gen_sub_mvr (size (rcons G x))) E) ++
+                                                   (rcons (substctx (under 1 sh1) G) (substh sh1 x)) ++ [:: v & D]).
+    move => Heq. rewrite Heq. rewrite - (cats1 _ (substh sh1 x)).
+    replace (substctx (under 1 sh1) G ++ [:: substh sh1 x]) with
+        (substctx sh1 (rcons G x)).
+    replace 
+       (subst
+          (under
+             (length
+                (substctx
+                   (gen_sub_mvr
+                      (size G)) E ++
+                 substctx sh1 G))
+             (dot (var 1)
+                (dot (var 0) (sh 2))))
+          (subst
+             (under (size E)
+                (gen_sub_mvr
+                   (size G))) a))
+ with
+           (subst
+              (under (size E)
+                     (gen_sub_mvr (size (rcons G x)))) a). apply X.
+    rewrite size_rcons. simpl. rewrite List.app_length.
+    repeat rewrite length_substctx.
+    rewrite compose_under. rewrite under_sum.
+    rewrite - subst_compose. auto.
+    rewrite - cats1. rewrite substctx_app. simpl. auto.
+    rewrite - (cats1 _ (substh sh1 x)).
+    rewrite - catA. rewrite (cat1s _ (v::D)). auto.
+    rewrite catA. auto.
+    rewrite size_rcons. auto.
+    rewrite size_cat. repeat rewrite size_substctx. auto.
+Qed.
+
+(*tests*)
+Lemma test1: forall (t: term False), subst (dot (var 1) (dot (var 0) (sh 2)))
+                                  (subst (under 1 (dot (var 1) (dot (var 0) (sh 2)))) t) =
+                            subst (gen_sub_mvl 2) t.
+intros. simpl. simpsub. simpl. auto. Qed.
+
+(*Lemma test2:
+  @subst False (dot (var 0) (sh 2)) (ppair (var 0)
+                                    (var 1)
+                             ) = subst sh1 (ppair (var 0)
+                                    (var 1)
+                                           ).
+  simpsub. simpl.*)
+
+Lemma move_list_r: forall E V G D m m' a,
+    tr ((substctx (gen_sub_mvr_list (size G) (size V)) E) ++
+        (substctx (sh (size V)) G) ++ V ++ D) (deq m m'
+                                                   (subst (under (size E)
+                                                      (gen_sub_mvr_list (size G) (size V))) a)
+                                                               ) (*need an under for a i think*)
+    -> tr (E ++ (substctx (sh (size G)) V)++ G ++ D)
+         (deq
+            (subst (under (size E) (gen_sub_mvl_list (size G) (size V))) m)
+            (subst (under (size E)  (gen_sub_mvl_list (size G) (size V))) m')
+                               a).
+  intros. move: m m' a G D E X. induction V using last_ind; intros; move: X; simpl; simpsub.
+ apply.
+  repeat rewrite size_rcons. simpl.
+  move => X. rewrite substctx_rcons.
+replace 
+    (E ++
+     rcons (substctx (under 1 (sh (size G))) V)
+       (substh (sh (size G)) x) ++ 
+       G ++ D) with
+    ((E ++ (substctx (under 1 (sh (size G))) V)) ++
+       (substh (sh (size G)) x::
+               (G ++ D))).
+rewrite !compose_under !under_sum !subst_compose !plusE. 
+replace (size E + size V) with
+    (size (E ++
+substctx (under 1 (sh (size G))) V
+    )). apply move_var_r.
+rewrite substctx_app.
+rewrite - substctx_compose. rewrite (substctx_eqsub (mvr_shift (size G)) ).
+replace (size G) with (size (substctx sh1 G)).
+remember (substctx
+        (under (size (substctx (under 1 (sh (size (substctx sh1 G)))) V))
+           (gen_sub_mvr (size (substctx sh1 G)))) E) as E'. 
+replace (size E) with (size E').
+rewrite - catA.
+apply IHV.
+repeat rewrite size_substctx. subst.
+simpsub. rewrite plusE.
+repeat rewrite size_substctx.
+replace 
+       
+       (subst
+          (compose
+             (under
+                (size
+                   (E ++
+                    substctx (dot (var 0) (sh (size G + 1))) V))
+                (gen_sub_mvr (size G)))
+             (under (size E)
+                (gen_sub_mvr_list (size G) (size V)))) a)
+ with
+           (subst
+              (under (size E)
+                 (compose
+                    (under 
+                       (size V)
+                       (gen_sub_mvr
+                        (size G)))
+                    (gen_sub_mvr_list
+                       (size G)
+                       (size V)))) a).
+replace 
+    (substctx
+       (compose (under (size V) (gen_sub_mvr (size G)))
+          (gen_sub_mvr_list (size G) (size V))) E ++
+       substctx (sh (1 + size V)) G ++ V ++ x :: D) with
+        (substctx
+           (compose (under (size V) (gen_sub_mvr (size G)))
+              (gen_sub_mvr_list (size G) (size V))) E ++
+         substctx (sh (size V).+1) G ++ rcons V x ++ D).
+apply X.
+rewrite - cats1. rewrite - (catA V [::x]). rewrite cat1s. auto.
+rewrite size_cat. rewrite - under_sum. rewrite - compose_under.
+rewrite size_substctx. auto. subst. 
+rewrite size_substctx. auto.
+rewrite size_substctx. auto.
+rewrite size_cat size_substctx. auto.
+rewrite - catA. rewrite cat_rcons. auto. Qed.
